Get the concrete test theory to build.

holsrcs/concrete_testsScript.sml
@@ -1,22 +1,39 @@
-open bossLib finite_mapTheory class_infoTheory
+open HolKernel Parse boolLib boolSimps
+open bossLib finite_mapTheory class_infoTheory pred_setTheory utilsTheory
 
 val _ = new_theory "concrete_tests"
 
-val s =
-  ``s with classmap updated_by
+val state1_def = Define`
+  state1 = ARB with classmap updated_by
       (\fm. fm |+ (Base "c",
                    SOME <| fields := [(FldDecl "foo" (Signed Char), F, Public);
                                       (FldDecl "bar" (Signed Int), F, Public)];
-                           ancestors := NONE |>))``;
+                           ancestors := NONE |>))
+`;
 
-val nsdmembers = SIMP_CONV (srw_ss()) [nsdmembers_def,
+val simp = SIMP_CONV (srw_ss()) [state1_def]
+
+val state1_applied_base = save_thm(
+  "state1_applied_base",
+  CONJ (simp ``state1.classmap ' (Base "c")``)
+       (simp ``deNONE state1.classmap ' (Base "c")``))
+val _ = export_rewrites ["state1_applied_base"]
+
+val base_in_classmap = store_thm(
+  "base_in_classmap",
+  ``Base "c" IN FDOM (deNONE state1.classmap) /\
+    Base "c" IN FDOM state1.classmap``,
+  SRW_TAC [][state1_def]);
+val _ = export_rewrites ["base_in_classmap"]
+
+val nsdmembers_state1 = SIMP_CONV (srw_ss()) [nsdmembers_def,
                                        finite_mapTheory.FLOOKUP_DEF]
-                           ``nsdmembers ^s (Base "c")``
+                           ``nsdmembers state1 (Base "c")``
 
 val layout = (SIMP_CONV (srw_ss()) [calc_subobjs] THENC
               ONCE_REWRITE_CONV [calc_rsubobjs] THENC
               SIMP_CONV (srw_ss()) [ancestor_def])
-             ``class_layout { so | (Base "c", so) IN subobjs ^s }``
+             ``class_layout { so | (Base "c", so) IN subobjs state1 }``
 
 val fmap_lemma = prove(
   ``!f. { c | ?v. c IN FDOM f /\ (f ' c = SOME v) } = FDOM (deNONE f)``,
@@ -32,11 +49,12 @@ val fmap_lemma = prove(
 
 val class_szmap = save_thm(
   "class_szmap",
-    SIMP_CONV (srw_ss()) [class_szmap_def, nsdmembers, layout,
-                          fmap_lemma, LET_THM,
+    SIMP_CONV (srw_ss()) [class_szmap_def, nsdmembers_state1, layout,
+                          fmap_lemma, LET_THM, base_in_classmap,
                           finite_mapTheory.FUN_FMAP_DEF]
-              ``class_szmap ^s ' (Base "c")``)
+              ``class_szmap state1 ' (Base "c")``)
 
+open memoryTheory
 val align_int = prove(``align m (Signed Int) a = (a = int_align)``,
                       ONCE_REWRITE_TAC [align_cases] THEN
                       SRW_TAC [][bit_align_def])
@@ -49,28 +67,28 @@ val sizeof_char = prove(``sizeof m (Signed Char) sz = (sz = 1)``,
                         SRW_TAC [][bit_size_def])
 
 val align_lemma = prove(
-  ``align (class_szmap ^s) (Class (Base "c")) a = (a = int_align)``,
+  ``align (class_szmap state1) (Class (Base "c")) a = (a = int_align)``,
   ONCE_REWRITE_TAC [align_cases] THEN
-  SIMP_TAC (srw_ss()) [class_szmap] THEN
+  SIMP_TAC (srw_ss()) [class_szmap, base_in_classmap] THEN
   SIMP_TAC (srw_ss() ++ DNF_ss) [align_int, align_char] THEN
   ASSUME_TAC int_align THEN DECIDE_TAC)
 
 val subobj_offset =
     (SIMP_CONV (srw_ss() ++ ARITH_ss)
                [subobj_offset_def, LET_THM,
-                genoffset_def, layout, nsdmembers,
+                genoffset_def, layout, nsdmembers_state1,
                 roundup_def, align_lemma, int_align])
-      ``subobj_offset ^s (Base "c") [Base "c"]``
+      ``subobj_offset state1 (Base "c") [Base "c"]``
 
 val nsds_bases = store_thm(
   "nsds_bases",
-  ``nsds_bases ^s (Base "c") = [(SOME "foo", Signed Char, 0);
-                                (SOME "bar", Signed Int, int_align)]``,
+  ``nsds_bases state1 (Base "c") = [(SOME "foo", Signed Char, 0);
+                                    (SOME "bar", Signed Int, int_align)]``,
 
-  SIMP_TAC (srw_ss()) [nsds_bases_def, nsdmembers, class_layout_def,
+  SIMP_TAC (srw_ss()) [nsds_bases_def, nsdmembers_state1, class_layout_def,
                        calc_subobjs] THEN
   ONCE_REWRITE_TAC [calc_rsubobjs] THEN
-  SIMP_TAC (srw_ss()) [ancestor_def] THEN
+  SIMP_TAC (srw_ss()) [ancestor_def, base_in_classmap] THEN
   SIMP_TAC (srw_ss()) [LET_THM, subobj_offset, align_int, align_char,
                        roundup_def, sizeof_char] THEN
   ASSUME_TAC int_align THEN
